# 解法1 迭代
```python
class Solution:
    def mergeTwoLists(self, l1: ListNode, l2: ListNode) -> ListNode:
        start = ListNode(0)
        l3 = start
        while l1 and l2:
            if l1.val > l2.val:
                l3.next = ListNode(l2.val)
                l3 = l3.next
                l2 = l2.next
            else:
                l3.next = ListNode(l1.val)
                l3 = l3.next
                l1 = l1.next
        if l1:
            l3.next = l1
        if l2:
            l3.next = l2
        return start.next
```

# 解法2 递归
```python
class Solution:
    def mergeTwoLists(self, l1: ListNode, l2: ListNode) -> ListNode:
        if not l1:
            return l2
        elif not l2:
            return l1
        elif l1.val > l2.val:
            l2.next = self.mergeTwoLists(l1, l2.next)
            return l2
        else:
            l1.next = self.mergeTwoLists(l1.next, l2)
            return l1
```